data/encodable.lean
@@ -79,6 +79,21 @@ instance option {α : Type*} [h : encodable α] : encodable (option α) :=
 @[simp] theorem decode_option_succ [encodable α] (n) :
   decode (option α) (succ n) = (decode α n).map some := rfl
 
+def decode2 (α) [encodable α] (n : ℕ) : option α :=
+(decode α n).bind (option.guard (λ a, encode a = n))
+
+theorem mem_decode2 [encodable α] {n : ℕ} {a : α} :
+  a ∈ decode2 α n ↔ a ∈ decode α n ∧ encode a = n :=
+by simp [decode2]; exact
+⟨λ ⟨_, h₁, rfl, h₂⟩, ⟨h₁, h₂⟩, λ ⟨h₁, h₂⟩, ⟨_, h₁, rfl, h₂⟩⟩
+
+theorem decode2_inj [encodable α] {n : ℕ} {a₁ a₂ : α}
+  (h₁ : a₁ ∈ decode2 α n) (h₂ : a₂ ∈ decode2 α n) : a₁ = a₂ :=
+encode_injective $ (mem_decode2.1 h₁).2.trans (mem_decode2.1 h₂).2.symm
+
+theorem encodek2 [encodable α] (a : α) : decode2 α (encode a) = some a :=
+mem_decode2.2 ⟨encodek _, rfl⟩
+
 section sum
 variables [encodable α] [encodable β]
 
