data/computability/halting.lean
@@ -1,0 +1,178 @@
+/-
+Copyright (c) 2018 Mario Carneiro. All rights reserved.
+Released under Apache 2.0 license as described in the file LICENSE.
+Author: Mario Carneiro
+
+More partial recursive functions using a universal program;
+Rice's theorem and the halting problem.
+-/
+import data.computability.partrec_code
+
+open encodable denumerable
+
+namespace nat.partrec
+open computable roption
+
+theorem merge' {f g}
+  (hf : nat.partrec f) (hg : nat.partrec g) :
+  ∃ h, nat.partrec h ∧ ∀ a,
+    (∀ x ∈ h a, x ∈ f a ∨ x ∈ g a) ∧
+    ((h a).dom ↔ (f a).dom ∨ (g a).dom) :=
+begin
+  rcases code.exists_code.1 hf with ⟨cf, rfl⟩,
+  rcases code.exists_code.1 hg with ⟨cg, rfl⟩,
+  have : nat.partrec (λ n,
+    (nat.rfind_opt (λ k, cf.evaln k n <|> cg.evaln k n))) :=
+  partrec.nat_iff.1 (partrec.rfind_opt $
+    primrec.option_orelse.to_comp.comp
+      (code.evaln_prim.to_comp.comp $ (snd.pair (const cf)).pair fst)
+      (code.evaln_prim.to_comp.comp $ (snd.pair (const cg)).pair fst)),
+  refine ⟨_, this, λ n, _⟩,
+  suffices, refine ⟨this,
+    ⟨λ h, (this _ ⟨h, rfl⟩).imp Exists.fst Exists.fst, _⟩⟩,
+  { intro h, rw nat.rfind_opt_dom,
+    simp [dom_iff_mem, code.evaln_complete] at h,
+    rcases h with ⟨x, k, e⟩ | ⟨x, k, e⟩,
+    { refine ⟨k, x, _⟩, simp [e] },
+    { refine ⟨k, _⟩,
+      cases cf.evaln k n with y,
+      { exact ⟨x, by simp [e]⟩ },
+      { exact ⟨y, by simp⟩ } } },
+  { intros x h,
+    rcases nat.rfind_opt_spec h with ⟨k, e⟩,
+    revert e,
+    simp; cases e' : cf.evaln k n with y; simp; intro,
+    { exact or.inr (code.evaln_sound e) },
+    { subst y,
+        exact or.inl (code.evaln_sound e') } }
+end
+
+end nat.partrec
+
+namespace partrec
+variables {α : Type*} {β : Type*} {γ : Type*} {σ : Type*}
+variables [primcodable α] [primcodable β] [primcodable γ] [primcodable σ]
+
+open computable roption nat.partrec (code) nat.partrec.code
+
+theorem merge' {f g : α →. σ}
+  (hf : partrec f) (hg : partrec g) :
+  ∃ k : α →. σ, partrec k ∧ ∀ a,
+    (∀ x ∈ k a, x ∈ f a ∨ x ∈ g a) ∧
+    ((k a).dom ↔ (f a).dom ∨ (g a).dom) :=
+let ⟨k, hk, H⟩ :=
+  nat.partrec.merge' (bind_decode2_iff.1 hf) (bind_decode2_iff.1 hg) in
+begin
+  let k' := λ a, (k (encode a)).bind (λ n, decode σ n),
+  refine ⟨k', ((nat_iff.2 hk).comp computable.encode).bind
+    (computable.decode.of_option.comp snd).to₂, λ a, _⟩,
+  suffices, refine ⟨this,
+    ⟨λ h, (this _ ⟨h, rfl⟩).imp Exists.fst Exists.fst, _⟩⟩,
+  { intro h, simp [k'],
+    have hk : (k (encode a)).dom :=
+      (H _).2.2 (by simpa [encodek2] using h),
+    existsi hk,
+    cases (H _).1 _ ⟨hk, rfl⟩ with h h;
+    { simp at h,
+      rcases h with ⟨a', ha', y, hy, e⟩,
+      simp [e.symm, encodek] } },
+  { intros x h', simp [k'] at h',
+    rcases h' with ⟨n, hn, hx⟩,
+    have := (H _).1 _ hn, simp [mem_decode2] at this,
+    cases this with h h;
+    { rcases h with ⟨a', ⟨ha₁, ha₂⟩, y, hy, rfl⟩,
+      rw encodek at hx ha₁, simp at hx ha₁, substs y a',
+      simp [hy] } },
+end
+
+theorem merge {f g : α →. σ}
+  (hf : partrec f) (hg : partrec g)
+  (H : ∀ a (x ∈ f a) (y ∈ g a), x = y) :
+  ∃ k : α →. σ, partrec k ∧ ∀ a x, x ∈ k a ↔ x ∈ f a ∨ x ∈ g a :=
+let ⟨k, hk, K⟩ := merge' hf hg in
+⟨k, hk, λ a x, ⟨(K _).1 _, λ h, begin
+  have : (k a).dom := (K _).2.2 (h.imp Exists.fst Exists.fst),
+  refine ⟨this, _⟩,
+  cases h with h h; cases (K _).1 _ ⟨this, rfl⟩ with h' h',
+  { exact mem_unique h' h },
+  { exact (H _ _ h _ h').symm },
+  { exact H _ _ h' _ h },
+  { exact mem_unique h' h }
+end⟩⟩
+
+theorem cond {c : α → bool} {f : α →. σ} {g : α →. σ}
+  (hc : computable c) (hf : partrec f) (hg : partrec g) :
+  partrec (λ a, cond (c a) (f a) (g a)) :=
+let ⟨cf, ef⟩ := exists_code.1 hf,
+    ⟨cg, eg⟩ := exists_code.1 hg in
+((eval_part.comp
+    (computable.cond hc (const cf) (const cg)) computable.id).bind
+  ((@computable.decode σ _).comp snd).of_option.to₂).of_eq $
+λ a, by cases c a; simp [ef, eg, encodek]
+
+theorem sum_cases
+  {f : α → β ⊕ γ} {g : α → β →. σ} {h : α → γ →. σ}
+  (hf : computable f) (hg : partrec₂ g) (hh : partrec₂ h) :
+  @partrec _ σ _ _ (λ a, sum.cases_on (f a) (g a) (h a)) :=
+option_some_iff.1 $ (cond
+  (sum_cases hf (const tt).to₂ (const ff).to₂)
+  (sum_cases_left hf (option_some_iff.2 hg).to₂ (const option.none).to₂)
+  (sum_cases_right hf (const option.none).to₂ (option_some_iff.2 hh).to₂))
+.of_eq $ λ a, by cases f a; simp
+
+end partrec
+
+def computable_pred {α} [primcodable α] (p : α → Prop) :=
+∃ [D : decidable_pred p],
+by exactI computable (λ a, to_bool (p a))
+
+/- recursively enumerable predicate -/
+def re_pred {α} [primcodable α] (p : α → Prop) :=
+partrec (λ a, roption.assert (p a) (λ _, roption.some ()))
+
+theorem computable_pred.of_eq {α} [primcodable α]
+  {p q : α → Prop}
+  (hp : computable_pred p) (H : ∀ a, p a ↔ q a) : computable_pred q :=
+(funext (λ a, propext (H a)) : p = q) ▸ hp
+
+namespace computable_pred
+variables {α : Type*} {σ : Type*}
+variables [primcodable α] [primcodable σ]
+open nat.partrec (code) nat.partrec.code computable
+
+theorem rice (C : set (ℕ →. ℕ))
+  (h : computable_pred (λ c, eval c ∈ C))
+  {f g} (hf : nat.partrec f) (hg : nat.partrec g)
+  (fC : f ∈ C) : g ∈ C :=
+begin
+  cases h with _ h, resetI,
+  rcases fixed_point₂ (partrec.cond (h.comp fst)
+    ((partrec.nat_iff.2 hg).comp snd).to₂
+    ((partrec.nat_iff.2 hf).comp snd).to₂).to₂ with ⟨c, e⟩,
+  simp at e,
+  by_cases eval c ∈ C,
+  { simp [h] at e, rwa ← e },
+  { simp at h, simp [h] at e,
+    rw e at h, contradiction }
+end
+
+theorem rice₂ (C : set code)
+  (H : ∀ cf cg, eval cf = eval cg → (cf ∈ C ↔ cg ∈ C)) :
+  computable_pred (λ c, c ∈ C) ↔ C = ∅ ∨ C = set.univ :=
+by haveI := classical.dec; exact
+have hC : ∀ f, f ∈ C ↔ eval f ∈ eval '' C,
+from λ f, ⟨set.mem_image_of_mem _, λ ⟨g, hg, e⟩, (H _ _ e).1 hg⟩,
+⟨λ h, or_iff_not_imp_left.2 $ λ C0,
+  set.eq_univ_of_forall $ λ cg,
+  let ⟨cf, fC⟩ := set.ne_empty_iff_exists_mem.1 C0 in
+  (hC _).2 $ rice (eval '' C) (h.of_eq hC)
+    (partrec.nat_iff.1 $ eval_part.comp (const cf) computable.id)
+    (partrec.nat_iff.1 $ eval_part.comp (const cg) computable.id)
+    ((hC _).1 fC),
+λ h, by rcases h with rfl | rfl; simp [computable_pred];
+  exact ⟨by apply_instance, computable.const _⟩⟩
+
+theorem halting_problem (n) : ¬ computable_pred (λ c, (eval c n).dom)
+| h := rice {f | (f n).dom} h nat.partrec.zero nat.partrec.none trivial
+
+end computable_pred
